theories/Labelled_Transition_System/Examples_of_LTS/VACCS/VACCS_Examples.v
@@ -29,7 +29,8 @@ From Stdlib.Wellfounded Require Import Inverse_Image.
 From stdpp Require Import base countable finite gmap list gmultiset strings.
 From TestingTheory Require Import InputOutputActions ActTau Must VACCS_Must_Characterization
 gLts Bisimulation Lts_OBA Lts_FW Lts_OBA_FB ParallelLTSConstruction
-InteractionBetweenLts Testing_Predicate DefinitionAS VACCS VACCS_Good VACCS_Instance.
+InteractionBetweenLts Testing_Predicate DefinitionAS VACCS VACCS_Good VACCS_Instance
+Convergence WeakTransitions Subset_Act MultisetLTSConstruction.
 
 (** ** VACCS **)
 (** *** Applications *)
