theories/Testing_Pre_orders/Must/Alternative_Preorder/Co_Inductive_Tower_Acceptance_Set/Coin_tower.v
@@ -392,25 +392,6 @@ Proof.
   now rewrite (leibniz_equiv _ _ HX).
 Qed.
 
-Global Instance Proper_lts_pre_co_actions `{gLtsEq P A} `{Γ : A -> PreAct}:
-  Proper ((eq_rel) ==> (≡)) (fun p => ⌈ Γ ⌉ (coR p)).
-Proof.
-  intros p p' Heq. intro μ_phi. split.
-  (* apply leibniz_equiv. intros Hyp. split. *)
-  - intro Hyp. destruct Hyp as (μ & mem_coR & eq);subst.
-    destruct mem_coR as (μ' & accepts & duo & b).
-    eapply accepts_preserved_by_eq in accepts;eauto.
-    assert (μ ∈ coR p') as mem.
-    { exists μ'. repeat split; eauto. }
-    eapply map_gamma_of_action;eauto.
-  - intro Hyp. destruct Hyp as (μ & mem_coR & eq);subst.
-    destruct mem_coR as (μ' & accepts & duo & b). symmetry in Heq.
-    eapply accepts_preserved_by_eq in accepts;eauto.
-    assert (μ ∈ coR p) as mem.
-    { exists μ'. repeat split; eauto. }
-    eapply map_gamma_of_action;eauto.
-Qed.
-
 Global Instance Proper_lts_stable `{gLtsEq P A}:
   Proper ((eq_rel) ==> (=) ==> (impl)) lts_refuses.
 Proof.
